books/centaur/gl/g-binary-+.lisp
@@ -24,12 +24,9 @@
              (equal yrd '(t))
              (equal xid '(t))
              (equal yid '(t)))
-        (let* ((rsum (+-ss nil xrn yrn))
-               (isum (+-ss nil xin yin)))
-          (mk-g-number
-           (if (boolean-listp rsum) (v2i rsum) rsum)
-           1
-           (if (boolean-listp isum) (v2i isum) isum)))
+        (let* ((rsum (bfr-+-ss nil xrn yrn))
+               (isum (bfr-+-ss nil xin yin)))
+          (mk-g-number rsum 1 isum))
       (g-apply 'binary-+ (gl-list x y)))))
 
 (in-theory (disable (g-binary-+-of-numbers)))
@@ -40,34 +37,34 @@
                   (equal (bfr-eval-list x env)
                          x))))
 
-(local (defthm rewrite-v2i-of-boolean-list
-         (implies (and (syntaxp (not (and (consp x)
-                                          (eq (car x) 'bfr-eval-list))))
-                       (bind-free '((env . (car env))) (env))
-                       (boolean-listp x))
-                  (equal (v2i x)
-                         (v2i (bfr-eval-list x env))))
-         :hints(("Goal" :in-theory (enable bfr-eval-list-when-boolean-listp)))
-         :rule-classes ((:rewrite :backchain-limit-lst 0))))
+;; (local (defthm rewrite-v2i-of-boolean-list
+;;          (implies (and (syntaxp (not (and (consp x)
+;;                                           (eq (car x) 'bfr-eval-list))))
+;;                        (bind-free '((env . (car env))) (env))
+;;                        (boolean-listp x))
+;;                   (equal (v2i x)
+;;                          (bfr-list->s x env)))
+;;          :hints(("Goal" :in-theory (enable bfr-eval-list-when-boolean-listp)))
+;;          :rule-classes ((:rewrite :backchain-limit-lst 0))))
 
-(local (defthm rewrite-v2n-of-boolean-list
-         (implies (and (syntaxp (not (and (consp x)
-                                          (eq (car x) 'bfr-eval-list))))
-                       (bind-free '((env . (car env))) (env))
-                       (boolean-listp x))
-                  (equal (v2n x)
-                         (v2n (bfr-eval-list x env))))
-         :hints(("Goal" :in-theory (enable bfr-eval-list-when-boolean-listp)))
-         :rule-classes ((:rewrite :backchain-limit-lst 0))))
+;; (local (defthm rewrite-v2n-of-boolean-list
+;;          (implies (and (syntaxp (not (and (consp x)
+;;                                           (eq (car x) 'bfr-eval-list))))
+;;                        (bind-free '((env . (car env))) (env))
+;;                        (boolean-listp x))
+;;                   (equal (v2n x)
+;;                          (bfr-list->u x env)))
+;;          :hints(("Goal" :in-theory (enable bfr-eval-list-when-boolean-listp)))
+;;          :rule-classes ((:rewrite :backchain-limit-lst 0))))
 
-(defthm bfr-eval-list-of-bfr-ite-bvv-fn-under-v2n
-  (equal (v2n (bfr-eval-list (bfr-ite-bvv-fn c a b) env))
-         (v2n (if (bfr-eval c env)
-                  (bfr-eval-list a env)
-                (bfr-eval-list b env))))
-  :hints(("Goal" :in-theory (enable bfr-ite-bvv-fn v2n)
-          :induct t)
-         (bfr-reasoning)))
+;; (defthm bfr-eval-list-of-bfr-ite-bvv-fn-unde
+;;   (equal (bfr-list->u (bfr-ite-bvv-fn c a b) env)
+;;          (if (bfr-eval c env)
+;;              (bfr-list->u a env)
+;;            (bfr-list->u b env))))
+;;   :hints(("Goal" :in-theory (enable bfr-ite-bvv-fn v2n)
+;;           :induct t)
+;;          (bfr-reasoning)))
 
 
 (local
@@ -113,7 +110,7 @@
   `(("goal" :in-theory (e/d* (general-concretep-atom
                               (:ruleset general-object-possibilities))
                              ((:definition ,gfn)
-                              i2v n2v v2i +-ss
+                              i2v n2v bfr-+-ss
                               general-numberp-eval-to-numberp
                               general-boolean-value-correct
                               bool-cond-itep-eval
